theories/datatypes.v
@@ -1,0 +1,219 @@
+(** Definition of Wasm datatypes **)
+(* (C) J. Pichon, M. Bodin - see LICENSE.txt *)
+
+Require Import common.
+Require Export numerics bytes.
+From mathcomp Require Import ssreflect ssrfun ssrnat ssrbool eqtype seq.
+
+Set Implicit Arguments.
+Unset Strict Implicit.
+Unset Printing Implicit Defensive.
+
+
+(* TODO: Documentation. *)
+
+
+Variable host : eqType. (* TODO: Do the same than for integers and floats. *)
+Variable host_state : eqType.
+
+Definition immediate := nat. (* i *)
+
+Definition static_offset := nat. (* off *)
+
+Definition alignment_exponent := nat. (* a *)
+
+
+(* TODO *)
+Parameter serialise_i32 : i32 -> bytes.
+Parameter serialise_i64 : i64 -> bytes.
+Parameter serialise_f32 : f32 -> bytes.
+Parameter serialise_f64 : f64 -> bytes.
+
+Definition mem := list byte.
+
+Inductive value_type : Type := (* t *)
+| T_i32
+| T_i64
+| T_f32
+| T_f64.
+
+Inductive packed_type : Type := (* tp *)
+| Tp_i8
+| Tp_i16
+| Tp_i32.
+
+Inductive mutability : Type := (* mut *)
+| T_immut
+| T_mut.
+
+Record global_type := (* tg *)
+  { tg_mut : mutability; tg_t : value_type }.
+
+Inductive function_type := (* tf *)
+| Tf : list value_type -> list value_type -> function_type.
+
+Record t_context := {
+  tc_types_t : list function_type;
+  tc_func_t : list function_type;
+  tc_global : list global_type;
+  tc_table : option nat;
+  tc_memory : option nat;
+  tc_local : list value_type;
+  tc_label : list (list value_type);
+  tc_return : option (list value_type);
+}.
+
+(* FIXME: Should we remove it?
+
+Record s_context := {
+  sc_inst : list t_context;
+  sc_funcs : list function_type;
+  sc_tab : list nat;
+  sc_mem : list nat;
+  sc_globs : list global_type;
+}.
+
+*)
+
+Inductive sx : Type :=
+| sx_S
+| sx_U.
+
+Inductive unop_i : Type :=
+| Clz
+| Ctz
+| Popcnt.
+
+Inductive unop_f : Type :=
+| Neg
+| Abs
+| Ceil
+| Floor
+| Trunc
+| Nearest
+| Sqrt.
+
+Inductive binop_i : Type :=
+| Add
+| Sub
+| Mul
+| Div : sx -> binop_i
+| Rem : sx -> binop_i
+| And
+| Or
+| Xor
+| Shl
+| Shr : sx -> binop_i
+| Rotl
+| Rotr.
+
+Inductive binop_f : Type :=
+| Addf
+| Subf
+| Mulf
+| Divf
+| Min
+| Max
+| Copysign.
+
+Inductive testop : Type :=
+| Eqz.
+
+Inductive relop_i : Type :=
+| Eq
+| Ne
+| Lt : sx -> relop_i
+| Gt : sx -> relop_i
+| Le : sx -> relop_i
+| Ge : sx -> relop_i.
+
+Inductive relop_f : Type :=
+| Eqf
+| Nef
+| Ltf
+| Gtf
+| Lef
+| Gef.
+
+Inductive cvtop : Type :=
+| Convert
+| Reinterpret.
+
+Inductive value : Type := (* v *)
+| ConstInt32 : i32 -> value
+| ConstInt64 : i64 -> value
+| ConstFloat32 : f32 -> value
+| ConstFloat64 : f64 -> value.
+
+Inductive basic_instruction : Type := (* be *)
+| Unreachable
+| Nop
+| Drop
+| Select
+| Block : function_type -> list basic_instruction -> basic_instruction
+| Loop : function_type -> list basic_instruction -> basic_instruction
+| If : function_type -> list basic_instruction -> list basic_instruction -> basic_instruction
+| Br : immediate -> basic_instruction
+| Br_if : immediate -> basic_instruction
+| Br_table : list immediate -> immediate -> basic_instruction
+| Return
+| Call : immediate -> basic_instruction
+| Call_indirect : immediate -> basic_instruction
+| Get_local : immediate -> basic_instruction
+| Set_local : immediate -> basic_instruction
+| Tee_local : immediate -> basic_instruction
+| Get_global : immediate -> basic_instruction
+| Set_global : immediate -> basic_instruction
+| Load : value_type -> option (packed_type * sx) -> alignment_exponent -> static_offset -> basic_instruction
+| Store : value_type -> option packed_type -> alignment_exponent -> static_offset -> basic_instruction
+| Current_memory
+| Grow_memory
+| EConst : value -> basic_instruction
+| Unop_i : value_type -> unop_i -> basic_instruction
+| Unop_f : value_type -> unop_f -> basic_instruction
+| Binop_i : value_type -> binop_i -> basic_instruction
+| Binop_f : value_type -> binop_f -> basic_instruction
+| Testop : value_type -> testop -> basic_instruction
+| Relop_i : value_type -> relop_i -> basic_instruction
+| Relop_f : value_type -> relop_f -> basic_instruction
+| Cvtop : value_type -> cvtop -> value_type -> option sx -> basic_instruction.
+
+Record instance : Type := (* inst *) {
+  i_types : list function_type;
+  i_funcs : list immediate;
+  i_tab : option immediate;
+  i_mem : option immediate;
+  i_globs : list immediate;
+}.
+
+Inductive function_closure : Type := (* cl *)
+| Func_native : instance -> function_type -> list value_type -> list basic_instruction -> function_closure
+| Func_host : function_type -> host -> function_closure.
+
+Definition tabinst := list (option function_closure).
+
+Record global : Type := {
+  g_mut : mutability;
+  g_val : value;
+}.
+
+Record store_record : Type := (* s *) {
+  s_funcs : list function_closure;
+  s_tab : list tabinst;
+  s_mem : list mem;
+  s_globs : list global;
+}.
+
+Inductive administrative_instruction : Type := (* e *)
+  | Basic : basic_instruction -> administrative_instruction
+  | Trap
+  | Callcl : function_closure -> administrative_instruction
+  | Label : nat -> seq administrative_instruction -> seq administrative_instruction -> administrative_instruction
+  | Local : nat -> instance -> list value -> seq administrative_instruction -> administrative_instruction
+  .
+
+Inductive lholed : Type :=
+  | LBase : list administrative_instruction -> list administrative_instruction -> lholed
+  | LRec : list administrative_instruction -> nat -> list administrative_instruction -> lholed -> list administrative_instruction -> lholed
+  .
+
