theories/datatypes_properties.v
@@ -1,0 +1,340 @@
+(** Properties about Wasm datatypes (mainly equality relations) **)
+(* (C) M. Bodin - see LICENSE.txt *)
+
+Require Import common.
+Require Export datatypes.
+From mathcomp Require Import ssreflect ssrfun ssrnat ssrbool eqtype seq.
+
+Set Implicit Arguments.
+Unset Strict Implicit.
+Unset Printing Implicit Defensive.
+
+
+Scheme Equality for value_type.
+Definition value_type_eqb v1 v2 : bool := value_type_eq_dec v1 v2.
+Definition eqvalue_typeP : Equality.axiom value_type_eqb :=
+  eq_dec_Equality_axiom value_type_eq_dec.
+
+Canonical Structure value_type_eqMixin := EqMixin eqvalue_typeP.
+Canonical Structure value_type_eqType := Eval hnf in EqType value_type value_type_eqMixin.
+
+Scheme Equality for packed_type.
+Definition packed_type_eqb v1 v2 : bool := packed_type_eq_dec v1 v2.
+Definition eqpacked_typeP : Equality.axiom packed_type_eqb :=
+  eq_dec_Equality_axiom packed_type_eq_dec.
+
+Canonical Structure packed_type_eqMixin := EqMixin eqpacked_typeP.
+Canonical Structure packed_type_eqType := Eval hnf in EqType packed_type packed_type_eqMixin.
+
+Scheme Equality for mutability.
+Definition mutability_eqb v1 v2 : bool := mutability_eq_dec v1 v2.
+Definition eqmutabilityP : Equality.axiom mutability_eqb :=
+  eq_dec_Equality_axiom mutability_eq_dec.
+
+Canonical Structure mutability_eqMixin := EqMixin eqmutabilityP.
+Canonical Structure mutability_eqType := Eval hnf in EqType mutability mutability_eqMixin.
+
+Scheme Equality for global_type.
+Definition global_type_eqb v1 v2 : bool := global_type_eq_dec v1 v2.
+Definition eqglobal_typeP : Equality.axiom global_type_eqb :=
+  eq_dec_Equality_axiom global_type_eq_dec.
+
+Canonical Structure global_type_eqMixin := EqMixin eqglobal_typeP.
+Canonical Structure global_type_eqType := Eval hnf in EqType global_type global_type_eqMixin.
+
+Definition function_type_eq_dec : forall tf1 tf2 : function_type,
+  {tf1 = tf2} + {tf1 <> tf2}.
+Proof. decidable_equality. Defined.
+
+Definition function_type_eqb v1 v2 : bool := function_type_eq_dec v1 v2.
+Definition eqfunction_typeP : Equality.axiom function_type_eqb :=
+  eq_dec_Equality_axiom function_type_eq_dec.
+
+Canonical Structure function_type_eqMixin := EqMixin eqfunction_typeP.
+Canonical Structure function_type_eqType :=
+  Eval hnf in EqType function_type function_type_eqMixin.
+
+Definition t_context_eq_dec : forall x y : t_context, {x = y} + {x <> y}.
+Proof. decidable_equality. Defined.
+
+Definition t_context_eqb v1 v2 : bool := t_context_eq_dec v1 v2.
+Definition eqt_contextP : Equality.axiom t_context_eqb :=
+  eq_dec_Equality_axiom t_context_eq_dec.
+
+Canonical Structure t_context_eqMixin := EqMixin eqt_contextP.
+Canonical Structure t_context_eqType := Eval hnf in EqType t_context t_context_eqMixin.
+
+Scheme Equality for sx.
+Definition sx_eqb v1 v2 : bool := sx_eq_dec v1 v2.
+Definition eqsxP : Equality.axiom sx_eqb :=
+  eq_dec_Equality_axiom sx_eq_dec.
+
+Canonical Structure sx_eqMixin := EqMixin eqsxP.
+Canonical Structure sx_eqType := Eval hnf in EqType sx sx_eqMixin.
+
+Scheme Equality for unop_i.
+Definition unop_i_eqb v1 v2 : bool := unop_i_eq_dec v1 v2.
+Definition equnop_iP : Equality.axiom unop_i_eqb :=
+  eq_dec_Equality_axiom unop_i_eq_dec.
+
+Canonical Structure unop_i_eqMixin := EqMixin equnop_iP.
+Canonical Structure unop_i_eqType := Eval hnf in EqType unop_i unop_i_eqMixin.
+
+Scheme Equality for unop_f.
+Definition unop_f_eqb v1 v2 : bool := unop_f_eq_dec v1 v2.
+Definition equnop_fP : Equality.axiom unop_f_eqb :=
+  eq_dec_Equality_axiom unop_f_eq_dec.
+
+Canonical Structure unop_f_eqMixin := EqMixin equnop_fP.
+Canonical Structure unop_f_eqType := Eval hnf in EqType unop_f unop_f_eqMixin.
+
+Scheme Equality for binop_i.
+Definition binop_i_eqb v1 v2 : bool := binop_i_eq_dec v1 v2.
+Definition eqbinop_iP : Equality.axiom binop_i_eqb :=
+  eq_dec_Equality_axiom binop_i_eq_dec.
+
+Canonical Structure binop_i_eqMixin := EqMixin eqbinop_iP.
+Canonical Structure binop_i_eqType := Eval hnf in EqType binop_i binop_i_eqMixin.
+
+Scheme Equality for binop_f.
+Definition binop_f_eqb v1 v2 : bool := binop_f_eq_dec v1 v2.
+Definition eqbinop_fP : Equality.axiom binop_f_eqb :=
+  eq_dec_Equality_axiom binop_f_eq_dec.
+
+Canonical Structure binop_f_eqMixin := EqMixin eqbinop_fP.
+Canonical Structure binop_f_eqType := Eval hnf in EqType binop_f binop_f_eqMixin.
+
+Scheme Equality for testop.
+Definition testop_eqb v1 v2 : bool := testop_eq_dec v1 v2.
+Definition eqtestopP : Equality.axiom testop_eqb :=
+  eq_dec_Equality_axiom testop_eq_dec.
+
+Canonical Structure testop_eqMixin := EqMixin eqtestopP.
+Canonical Structure testop_eqType := Eval hnf in EqType testop testop_eqMixin.
+
+Scheme Equality for relop_i.
+Definition relop_i_eqb v1 v2 : bool := relop_i_eq_dec v1 v2.
+Definition eqrelop_iP : Equality.axiom relop_i_eqb :=
+  eq_dec_Equality_axiom relop_i_eq_dec.
+
+Canonical Structure relop_i_eqMixin := EqMixin eqrelop_iP.
+Canonical Structure relop_i_eqType := Eval hnf in EqType relop_i relop_i_eqMixin.
+
+Scheme Equality for relop_f.
+Definition relop_f_eqb v1 v2 : bool := relop_f_eq_dec v1 v2.
+Definition eqrelop_fP : Equality.axiom relop_f_eqb :=
+  eq_dec_Equality_axiom relop_f_eq_dec.
+
+Canonical Structure relop_f_eqMixin := EqMixin eqrelop_fP.
+Canonical Structure relop_f_eqType := Eval hnf in EqType relop_f relop_f_eqMixin.
+
+Scheme Equality for cvtop.
+Definition cvtop_eqb v1 v2 : bool := cvtop_eq_dec v1 v2.
+Definition eqcvtopP : Equality.axiom cvtop_eqb :=
+  eq_dec_Equality_axiom cvtop_eq_dec.
+
+Canonical Structure cvtop_eqMixin := EqMixin eqcvtopP.
+Canonical Structure cvtop_eqType := Eval hnf in EqType cvtop cvtop_eqMixin.
+
+Definition value_eq_dec : forall v1 v2 : value, {v1 = v2} + {v1 <> v2}.
+Proof. decidable_equality. Defined.
+
+Definition value_eqb v1 v2 : bool := value_eq_dec v1 v2.
+Definition eqvalueP : Equality.axiom value_eqb :=
+  eq_dec_Equality_axiom value_eq_dec.
+
+Canonical Structure value_eqMixin := EqMixin eqvalueP.
+Canonical Structure value_eqType := Eval hnf in EqType value value_eqMixin.
+
+(* TODO: [basic_instruction_rect'] *)
+
+(* TODO:
+Scheme Equality for basic_instruction.
+Definition eqglobal_typeP := eq_dec_Equality_axiom global_type_eq_dec.
+*)
+Parameter basic_instruction_eqb : basic_instruction -> basic_instruction -> bool.
+
+Parameter eqbasic_instructionP : Equality.axiom basic_instruction_eqb.
+
+Canonical Structure basic_instruction_eqMixin := EqMixin eqbasic_instructionP.
+Canonical Structure basic_instruction_eqType :=
+  Eval hnf in EqType basic_instruction basic_instruction_eqMixin.
+
+Definition instance_eq_dec : forall (i1 i2 : instance), {i1 = i2} + {i1 <> i2}.
+Proof. decidable_equality. Defined.
+
+Definition instance_eqb i1 i2 : bool := instance_eq_dec i1 i2.
+
+Definition eqinstanceP : Equality.axiom instance_eqb :=
+  eq_dec_Equality_axiom instance_eq_dec.
+
+Canonical Structure instance_eqMixin := EqMixin eqinstanceP.
+Canonical Structure instance_eqType := Eval hnf in EqType instance instance_eqMixin.
+
+Definition function_closure_eq_dec : forall (cl1 cl2 : function_closure),
+  {cl1 = cl2} + {cl1 <> cl2}.
+Proof. decidable_equality. Defined.
+
+Definition function_closure_eqb cl1 cl2 : bool := function_closure_eq_dec cl1 cl2.
+Definition eqfunction_closureP : Equality.axiom function_closure_eqb :=
+  eq_dec_Equality_axiom function_closure_eq_dec.
+
+Canonical Structure function_closure_eqMixin := EqMixin eqfunction_closureP.
+Canonical Structure function_closure_eqType :=
+  Eval hnf in EqType function_closure function_closure_eqMixin.
+
+Definition global_eq_dec : forall v1 v2 : global, {v1 = v2} + {v1 <> v2}.
+Proof. decidable_equality. Defined.
+
+Definition global_eqb v1 v2 : bool := global_eq_dec v1 v2.
+Definition eqglobalP : Equality.axiom global_eqb :=
+  eq_dec_Equality_axiom global_eq_dec.
+
+Canonical Structure global_eqMixin := EqMixin eqglobalP.
+Canonical Structure global_eqType := Eval hnf in EqType global global_eqMixin.
+
+Definition store_record_eq_dec : forall v1 v2 : store_record, {v1 = v2} + {v1 <> v2}.
+Proof. decidable_equality. Defined.
+
+Definition store_record_eqb v1 v2 : bool := store_record_eq_dec v1 v2.
+Definition eqstore_recordP : Equality.axiom store_record_eqb :=
+  eq_dec_Equality_axiom store_record_eq_dec.
+
+Canonical Structure store_record_eqMixin := EqMixin eqstore_recordP.
+Canonical Structure store_record_eqType := Eval hnf in EqType store_record store_record_eqMixin.
+
+(** Induction scheme for [administrative_instruction]. **)
+Section administrative_instruction_rect'.
+
+  Variable P : administrative_instruction -> Type.
+
+  Hypothesis basic : forall b, P (Basic b).
+  Hypothesis trap : P Trap.
+  Hypothesis callcl : forall f, P (Callcl f).
+  Hypothesis label : forall n es1 es2,
+    TProp.Forall P es1 ->
+    TProp.Forall P es2 ->
+    P (Label n es1 es2).
+  Hypothesis local : forall n i vs es,
+    TProp.Forall P es ->
+    P (Local n i vs es).
+
+  Fixpoint administrative_instruction_rect' e : P e :=
+    let rect_list :=
+      fix rect_list es : TProp.Forall P es :=
+        match es with
+        | [::] => TProp.Forall_nil _
+        | e :: l => TProp.Forall_cons (administrative_instruction_rect' e) (rect_list l)
+        end in
+    match e with
+    | Basic b => basic b
+    | Trap => trap
+    | Callcl f => callcl f
+    | Label n es1 es2 => label n (rect_list es1) (rect_list es2)
+    | Local n i vs es => local n i vs (rect_list es)
+    end.
+
+End administrative_instruction_rect'.
+
+Definition administrative_instruction_ind' (P : administrative_instruction -> Prop) :=
+  @administrative_instruction_rect' P.
+
+Fixpoint administrative_instruction_eqb (e1 e2 : administrative_instruction) : bool :=
+  let fff :=
+      (fix f (l1 l2 : list administrative_instruction) :=
+         match l1, l2 with
+         | nil, nil => true
+         | cons _ _, nil => false
+         | nil, cons _ _ => false
+         | cons x xs, cons y ys => (administrative_instruction_eqb x y) && (f xs ys)
+         end
+      ) in
+  match e1, e2 with
+  | Basic be1, Basic be2 => be1 == be2
+  | Trap, Trap => true
+  | Callcl cl1, Callcl cl2 => cl1 == cl2
+  | Label n1 es11 es12, Label n2 es21 es22 =>
+    (Nat.eqb n1 n2) &&
+    (fff es11 es21) &&
+    (fff es12 es22)
+  | Local n1 i1 vs1 es1, Local n2 i2 vs2 es2 =>
+    (Nat.eqb n1 n2) &&
+    (instance_eqb i1 i2) &&
+    (vs1 == vs2) &&
+    (fff es1 es2)
+  | _, _ => false
+  end.
+
+Lemma eqadministrative_instructionP : Equality.axiom administrative_instruction_eqb.
+Proof.
+  assert (IH: forall es es',
+    TProp.Forall (fun x => forall y, reflect (x = y) (administrative_instruction_eqb x y)) es ->
+    reflect (es = es')
+      ((fix f (l1 l2 : list administrative_instruction) :=
+         match l1, l2 with
+         | nil, nil => true
+         | cons _ _, nil => false
+         | nil, cons _ _ => false
+         | cons x xs, cons y ys => (administrative_instruction_eqb x y) && (f xs ys)
+         end) es es')).
+  { elim.
+    - case.
+      + move=> IH. by apply ReflectT.
+      + move=> a l IH. by apply ReflectF.
+    - move=> a l IH. case.
+      + move=> IH'. by apply ReflectF.
+      + move=> a' l' IH'. inversion_clear IH' as [|? ? IH1 IH2].
+        eapply iffP; first by apply andP.
+        * case => ? ?. f_equal.
+          -- by apply/IH1.
+          -- by apply/IH.
+        * case=> ? ?. split.
+          -- by apply/IH1.
+          -- by apply/IH.
+  }
+  move=> x. induction x using administrative_instruction_rect';
+    move=> y; destruct y; simpl;
+    try (apply ReflectF; discriminate).
+  - eapply iffP; first by apply/eqP.
+    + by elim.
+    + by case.
+  - by apply ReflectT.
+  - eapply iffP; first by apply/eqP.
+    + by elim.
+    + by case.
+  - apply iffP with (P := n = n0 /\ es1 = l /\ es2 = l0).
+    + move: (IH es1 l X) (IH es2 l0 X0) => {IH X X0} R1 R2.
+      eapply iffP; first by apply andP.
+      * case. move/andP. case=> ? ? ?. split; first by apply/eqP.
+        split; first by apply/R1. by apply/R2.
+      * intros (?&?&?). subst. split; last by apply/R2.
+        apply/andP. split; last by apply/R1. by apply/eqP.
+    + by repeat (case; elim).
+    + by case.
+  - apply iffP with (P := n = n0 /\ i = i0 /\ vs = l /\ es = l0).
+    + move: (IH es l0 X) => {IH X} R.
+      eapply iffP; first by apply andP.
+      * case. move/andP. case. move/andP. case=> ? ? ? ?.
+        repeat (split; first by apply/eqP). by apply/R.
+      * intros (?&?&?&?). subst. split; last by apply/R.
+        apply/andP. split; last by apply/eqP.
+        apply/andP. split; first by apply/eqP.
+        by apply/eqinstanceP.
+    + by repeat (case; elim).
+    + by case.
+Qed.
+
+Canonical Structure administrative_instruction_eqMixin := EqMixin eqadministrative_instructionP.
+Canonical Structure administrative_instruction_eqType :=
+  Eval hnf in EqType administrative_instruction administrative_instruction_eqMixin.
+
+Definition lholed_eq_dec : forall v1 v2 : lholed, {v1 = v2} + {v1 <> v2}.
+Proof. decidable_equality. Defined.
+
+Definition lholed_eqb v1 v2 : bool := lholed_eq_dec v1 v2.
+Definition eqlholedP : Equality.axiom lholed_eqb :=
+  eq_dec_Equality_axiom lholed_eq_dec.
+
+Canonical Structure lholed_eqMixin := EqMixin eqlholedP.
+Canonical Structure lholed_eqType := Eval hnf in EqType lholed lholed_eqMixin.
+
