theories/operations.v
@@ -1,0 +1,487 @@
+(** Basic operations over Wasm datatypes **)
+(* (C) J. Pichon, M. Bodin - see LICENSE.txt *)
+
+Require Import common.
+From mathcomp Require Import ssreflect ssrfun ssrnat ssrbool eqtype seq.
+Require Export datatypes_properties.
+
+Set Implicit Arguments.
+Unset Strict Implicit.
+Unset Printing Implicit Defensive.
+
+
+Definition read_bytes (m : mem) (n : nat) (l : nat) : bytes :=
+  take l (List.skipn n m).
+
+Definition write_bytes (m : mem) (n : nat) (bs : bytes) : mem :=
+  app (take n m) (app bs (List.skipn (n + length bs) m)).
+
+Definition mem_append (m : mem) (bs : bytes) := app m bs.
+
+Definition upd_s_mem (s : store_record) (m : list mem) : store_record :=
+  Build_store_record
+    (s_funcs s)
+    (s_tab s)
+    m
+    (s_globs s).
+
+Definition mem_size (m : mem) :=
+  length m.
+
+Definition mem_grow (m : mem) (n : nat) :=
+  m ++ bytes_replicate (n * 64000) #00.
+
+(* TODO: We crucially need documentation here. *)
+
+Definition load (m : mem) (n : nat) (off : static_offset) (l : nat) : option bytes :=
+  if mem_size m >= (n + off + l)
+  then Some (read_bytes m (n + off) l)
+  else None.
+
+Definition sign_extend (s : sx) (l : nat) (bs : bytes) : bytes :=
+  (* TODO *) bs.
+(* TODO
+  let msb := msb (msbyte bytes) in
+  let byte := (match sx with sx_U => O | sx_S => if msb then -1 else 0) in
+  bytes_takefill byte l bytes
+*)
+
+Definition load_packed (s : sx) (m : mem) (n : nat) (off : static_offset) (lp : nat) (l : nat) : option bytes :=
+  option_map (sign_extend s l) (load m n off lp).
+
+Definition store (m : mem) (n : nat) (off : static_offset) (bs : bytes) (l : nat) : option mem :=
+  if (mem_size m) >= (n + off + l)
+  then Some (write_bytes m (n + off) (bytes_takefill #00 l bs))
+  else None.
+
+Definition store_packed := store.
+
+(* TODO: The whole host should be defined as a mixin in a separate file. *)
+Parameter wasm_deserialise : bytes -> value_type -> value.
+
+Parameter host_apply : store_record -> function_type -> datatypes.host -> list value -> datatypes.host_state -> option (store_record * list value).
+
+Definition typeof (v : value) : value_type :=
+  match v with
+  | ConstInt32 _ => T_i32
+  | ConstInt64 _ => T_i64
+  | ConstFloat32 _ => T_f32
+  | ConstFloat64 _ => T_f64
+  end.
+
+Definition option_projl (A B : Type) (x : option (A * B)) : option A :=
+  option_map fst x.
+
+Definition option_projr (A B : Type) (x : option (A * B)) : option B :=
+  option_map snd x.
+
+Definition t_length (t : value_type) : nat :=
+  match t with
+  | T_i32 => 4
+  | T_i64 => 8
+  | T_f32 => 4
+  | T_f64 => 8
+  end.
+
+Definition tp_length (tp : packed_type) : nat :=
+  match tp with
+  | Tp_i8 => 1
+  | Tp_i16 => 2
+  | Tp_i32 => 4
+  end.
+
+Definition is_int_t (t : value_type) : bool :=
+  match t with
+  | T_i32 => true
+  | T_i64 => true
+  | T_f32 => false
+  | T_f64 => false
+  end.
+
+Definition is_float_t (t : value_type) : bool :=
+  match t with
+  | T_i32 => false
+  | T_i64 => false
+  | T_f32 => true
+  | T_f64 => true
+  end.
+
+Definition is_mut (tg : global_type) : bool :=
+  tg_mut tg == T_mut.
+
+
+Definition app_unop_i (e : Wasm_int.type) (iop : unop_i) : Wasm_int.sort e -> Wasm_int.sort e :=
+  let: Wasm_int.Pack u (Wasm_int.Class eqmx intmx) as e' := e
+    return Wasm_int.sort e' -> Wasm_int.sort e' in
+  match iop with
+  | Ctz => Wasm_int.int_ctz intmx
+  | Clz => Wasm_int.int_clz intmx
+  | Popcnt => Wasm_int.int_popcnt intmx
+  end.
+
+Definition app_unop_f (e : Wasm_float.type) (fop : unop_f) : Wasm_float.sort e -> Wasm_float.sort e :=
+  let: Wasm_float.Pack u (Wasm_float.Class eqmx mx) as e' := e
+    return Wasm_float.sort e' -> Wasm_float.sort e' in
+  match fop with
+  | Neg => Wasm_float.float_neg mx
+  | Abs => Wasm_float.float_abs mx
+  | Ceil => Wasm_float.float_ceil mx
+  | Floor => Wasm_float.float_floor mx
+  | Trunc => Wasm_float.float_trunc mx
+  | Nearest => Wasm_float.float_nearest mx
+  | Sqrt => Wasm_float.float_sqrt mx
+  end.
+
+Definition app_binop_i (e : Wasm_int.type) (iop : binop_i)
+    : Wasm_int.sort e -> Wasm_int.sort e -> option (Wasm_int.sort e) :=
+  let: Wasm_int.Pack u (Wasm_int.Class _ mx) as e' := e
+    return Wasm_int.sort e' -> Wasm_int.sort e' -> option (Wasm_int.sort e') in
+  let: add_some := fun f c1 c2 => Some (f c1 c2) in
+  match iop with
+  | Add => add_some (Wasm_int.int_add mx)
+  | Sub => add_some (Wasm_int.int_sub mx)
+  | Mul => add_some (Wasm_int.int_mul mx)
+  | Div sx_U => Wasm_int.int_div_u mx
+  | Div sx_S => Wasm_int.int_div_s mx
+  | Rem sx_U => Wasm_int.int_rem_u mx
+  | Rem sx_S => Wasm_int.int_rem_s mx
+  | And => add_some (Wasm_int.int_and mx)
+  | Or => add_some (Wasm_int.int_or mx)
+  | Xor => add_some (Wasm_int.int_xor mx)
+  | Shl => add_some (Wasm_int.int_shl mx)
+  | Shr sx_U => add_some (Wasm_int.int_shr_u mx)
+  | Shr sx_S => add_some (Wasm_int.int_shr_s mx)
+  | Rotl => add_some (Wasm_int.int_rotl mx)
+  | Rotr => add_some (Wasm_int.int_rotr mx)
+  end.
+
+Definition app_binop_f (e : Wasm_float.type) (fop : binop_f)
+    : Wasm_float.sort e -> Wasm_float.sort e -> option (Wasm_float.sort e) :=
+  let: Wasm_float.Pack u (Wasm_float.Class _ mx) as e' := e
+    return Wasm_float.sort e' -> Wasm_float.sort e' -> option (Wasm_float.sort e') in
+  let: add_some := fun f c1 c2 => Some (f c1 c2) in
+  match fop with
+  | Addf => add_some (Wasm_float.float_add mx)
+  | Subf => add_some (Wasm_float.float_sub mx)
+  | Mulf => add_some (Wasm_float.float_mul mx)
+  | Divf => add_some (Wasm_float.float_div mx)
+  | Min => add_some (Wasm_float.float_min mx)
+  | Max => add_some (Wasm_float.float_max mx)
+  | Copysign => add_some (Wasm_float.float_copysign mx)
+  end.
+
+Definition app_testop_i (e : Wasm_int.type) (o : testop) : Wasm_int.sort e -> bool :=
+  let: Wasm_int.Pack u (Wasm_int.Class _ mx) as e' := e return Wasm_int.sort e' -> bool in
+  match o with
+  | Eqz => Wasm_int.int_eqz mx
+  end.
+
+Definition app_relop_i (e : Wasm_int.type) (rop : relop_i)
+    : Wasm_int.sort e -> Wasm_int.sort e -> bool :=
+  let: Wasm_int.Pack u (Wasm_int.Class _ mx) as e' := e
+    return Wasm_int.sort e' -> Wasm_int.sort e' -> bool in
+  match rop with
+  | Eq => Wasm_int.int_eq mx
+  | Ne => @Wasm_int.int_ne _
+  | Lt sx_U => Wasm_int.int_lt_u mx
+  | Lt sx_S => Wasm_int.int_lt_s mx
+  | Gt sx_U => Wasm_int.int_gt_u mx
+  | Gt sx_S => Wasm_int.int_gt_s mx
+  | Le sx_U => Wasm_int.int_le_u mx
+  | Le sx_S => Wasm_int.int_le_s mx
+  | Ge sx_U => Wasm_int.int_ge_u mx
+  | Ge sx_S => Wasm_int.int_ge_s mx
+  end.
+
+Definition app_relop_f (e : Wasm_float.type) (rop : relop_f)
+    : Wasm_float.sort e -> Wasm_float.sort e -> bool :=
+  let: Wasm_float.Pack u (Wasm_float.Class _ mx) as e' := e
+    return Wasm_float.sort e' -> Wasm_float.sort e' -> bool in
+  match rop with
+  | Eqf => Wasm_float.float_eq mx
+  | Nef => @Wasm_float.float_ne _
+  | Ltf => Wasm_float.float_lt mx
+  | Gtf => Wasm_float.float_gt mx
+  | Lef => Wasm_float.float_le mx
+  | Gef => Wasm_float.float_ge mx
+  end.
+
+Definition types_agree (t : value_type) (v : value) : bool :=
+  (typeof v) == t.
+
+Definition cl_type (cl : function_closure) : function_type :=
+  match cl with
+  | Func_native _ tf _ _ => tf
+  | Func_host tf _ => tf
+  end.
+
+Definition rglob_is_mut (g : global) : bool :=
+  g_mut g == T_mut.
+
+Definition option_bind (A B : Type) (f : A -> option B) (x : option A) :=
+  match x with
+  | None => None
+  | Some y => f y
+  end.
+
+Definition stypes (s : store_record) (i : instance) (j : nat) : option function_type :=
+  List.nth_error (i_types i) j.
+(* TODO: optioned *)
+
+Definition sfunc_ind (s : store_record) (i : instance) (j : nat) : option nat :=
+  List.nth_error (i_funcs i) j.
+
+Definition sfunc (s : store_record) (i : instance) (j : nat) : option function_closure :=
+  option_bind (List.nth_error (s_funcs s)) (sfunc_ind s i j).
+
+Definition sglob_ind (s : store_record) (i : instance) (j : nat) : option nat :=
+  List.nth_error (i_globs i) j.
+
+Definition sglob (s : store_record) (i : instance) (j : nat) : option global :=
+  option_bind (List.nth_error (s_globs s))
+    (sglob_ind s i j).
+
+Definition sglob_val (s : store_record) (i : instance) (j : nat) : option value :=
+  option_map g_val (sglob s i j).
+
+Definition smem_ind (s : store_record) (i : instance) : option nat :=
+  i_mem i.
+
+Definition stab_s (s : store_record) (i j : nat) : option function_closure :=
+  let stabinst := List.nth_error (s_tab s) i in
+  option_bind (fun x => x) (
+  option_bind
+    (fun stabinst => if length stabinst > j then List.nth_error stabinst j else None)
+    stabinst).
+
+Definition stab (s : store_record) (i : instance) (j : nat) : option function_closure :=
+  if i_tab i is Some k then stab_s s k j else None.
+
+Definition update_list_at {A : Type} (l : list A) (k : nat) (a : A) :=
+  take k l ++ [::a] ++ List.skipn (k + 1) l.
+
+Definition supdate_glob_s (s : store_record) (k : nat) (v : value) : option store_record :=
+  option_map
+    (fun g =>
+      let g' := Build_global (g_mut g) v in
+      let gs' := update_list_at (s_globs s) k g' in
+      Build_store_record (s_funcs s) (s_tab s) (s_mem s) gs')
+    (List.nth_error (s_globs s) k).
+
+Definition supdate_glob (s : store_record) (i : instance) (j : nat) (v : value) : option store_record :=
+  option_bind
+    (fun k => supdate_glob_s s k v)
+    (sglob_ind s i j).
+
+Definition is_const (e : administrative_instruction) : bool :=
+  if e is Basic _ then true else false.
+
+Definition const_list (es : list administrative_instruction) : bool :=
+  List.forallb is_const es.
+
+Definition store_extension (s s' : store_record) : bool :=
+  (s_funcs s == s_funcs s') &&
+  (s_tab s == s_tab s') &&
+  (all2 (fun bs bs' => mem_size bs <= mem_size bs') (s_mem s) (s_mem s')) &&
+  (s_globs s == s_globs s').
+
+Definition to_e_list (bes : list basic_instruction) : list administrative_instruction :=
+  map Basic bes.
+
+(** [v_to_e_list]: some kind of the opposite of [split_vals_e] (see [interperter.v]:
+    takes a list of [v] and gives back a list where each [v] is mapped to [Basic (EConst v)]. **)
+Definition v_to_e_list (ves : list value) : list administrative_instruction :=
+  map (fun v => Basic (EConst v)) ves.
+
+Fixpoint lfill (k : nat) (lh : lholed) (es : list administrative_instruction) : option (list administrative_instruction) :=
+  match k with
+  | 0 =>
+    if lh is LBase vs es' then
+      if const_list vs then Some (app vs (app es es')) else None
+    else None
+  | k'.+1 =>
+    if lh is LRec vs n es' lh' es'' then
+      if const_list vs then
+        if lfill k' lh' es is Some lfilledk then
+          Some (app vs (cons (Label n es' lfilledk) es''))
+        else None
+      else None
+    else None
+  end.
+
+Definition lfilled (k : nat) (lh : lholed) (es : list administrative_instruction) (es' : list administrative_instruction) : bool :=
+  if lfill k lh es is Some es'' then es' == es'' else false.
+
+Inductive lfilledInd : nat -> lholed -> list administrative_instruction -> list administrative_instruction -> Prop :=
+| LfilledBase: forall vs es es',
+    const_list vs ->
+    lfilledInd 0 (LBase vs es') es (vs ++ es ++ es')
+| LfilledRec: forall k vs n es' lh' es'' es LI,
+    const_list vs ->
+    lfilledInd k lh' es LI ->
+    lfilledInd (k.+1) (LRec vs n es' lh' es'') es (vs ++ [ :: (Label n es' LI) ] ++ es'').
+
+Lemma lfilled_Ind_Equivalent: forall k lh es LI,
+    lfilled k lh es LI <-> lfilledInd k lh es LI.
+Proof.
+  move => k. split.
+  - move: lh es LI. induction k; move => lh es LI HFix.
+    + unfold lfilled in HFix. simpl in HFix. destruct lh => //=.
+      * destruct (const_list l) eqn:HConst => //=.
+        { replace LI with (l++es++l0); first by apply LfilledBase.
+          symmetry. move: HFix. by apply/eqseqP. }
+    + unfold lfilled in HFix. simpl in HFix. destruct lh => //=.
+      * destruct (const_list l) eqn:HConst => //=.
+        { destruct (lfill k lh es) eqn:HLF => //=.
+          { replace LI with (l ++ [ :: (Label n l0 l2)] ++ l1).
+          apply LfilledRec; first by [].
+          apply IHk. unfold lfilled; first by rewrite HLF.
+          symmetry. move: HFix. by apply/eqseqP. }
+        }
+  - move => HLF. induction HLF.
+    + unfold lfilled. unfold lfill. by rewrite H.
+    + unfold lfilled. unfold lfill. rewrite H. fold lfill.
+      unfold lfilled in IHHLF. destruct (lfill k lh' es) => //=.
+      * replace LI with l => //=.
+        symmetry. by apply/eqseqP.
+Qed.
+
+Lemma lfilledP: forall k lh es LI,
+    reflect (lfilledInd k lh es LI) (lfilled k lh es LI).
+Proof.
+  move => k lh es LI. destruct (lfilled k lh es LI) eqn:HLFBool.
+  - apply ReflectT. by apply lfilled_Ind_Equivalent.
+  - apply ReflectF. move=> HContra. apply lfilled_Ind_Equivalent in HContra.
+    by rewrite HLFBool in HContra.
+Qed.
+
+Fixpoint lfill_exact (k : nat) (lh : lholed) (es : list administrative_instruction) : option (list administrative_instruction) :=
+  match k with
+  | 0 =>
+    if lh is LBase nil nil then Some es else None
+  | k'.+1 =>
+    if lh is LRec vs n es' lh' es'' then
+      if const_list vs then
+        if lfill_exact k' lh' es is Some lfilledk then
+          Some (app vs (cons (Label n es' lfilledk) es''))
+        else None
+      else None
+    else None
+  end.
+
+Definition lfilled_exact (k : nat) (lh : lholed) (es : list administrative_instruction) (es' : list administrative_instruction) : bool :=
+  if lfill_exact k lh es is Some es'' then es' == es'' else false.
+
+Definition load_store_t_bounds (a : alignment_exponent) (tp : option packed_type) (t : value_type) : bool :=
+  match tp with
+  | None => Nat.pow 2 a <= t_length t
+  | Some tp' => (Nat.pow 2 a <= tp_length tp') && (tp_length tp' < t_length t) && (is_int_t t)
+  end.
+
+Definition cvt_i32 (s : option sx) (v : value) : option i32 :=
+  match v with
+  | ConstInt32 _ => None
+  | ConstInt64 c => Some (wasm_wrap c)
+  | ConstFloat32 c =>
+    match s with
+    | Some sx_U => Wasm_float.float_ui32_trunc f32m c
+    | Some sx_S => Wasm_float.float_ui32_trunc f32m c
+    | None => None
+    end
+  | ConstFloat64 c =>
+    match s with
+    | Some sx_U => Wasm_float.float_ui32_trunc f64m c
+    | Some sx_S => Wasm_float.float_ui32_trunc f64m c
+    | None => None
+    end
+  end.
+
+Definition cvt_i64 (s : option sx) (v : value) : option i64 :=
+  match v with
+  | ConstInt32 c =>
+    match s with
+    | Some sx_U => Some (wasm_extend_u c)
+    | Some sx_S => Some (wasm_extend_s c)
+    | None => None
+    end
+  | ConstInt64 c => None
+  | ConstFloat32 c =>
+    match s with
+    | Some sx_U => Wasm_float.float_ui64_trunc f32m c
+    | Some sx_S => Wasm_float.float_si64_trunc f32m c
+    | None => None
+    end
+  | ConstFloat64 c =>
+    match s with
+    | Some sx_U => Wasm_float.float_ui64_trunc f64m c
+    | Some sx_S => Wasm_float.float_si64_trunc f64m c
+    | None => None
+    end
+  end.
+
+Definition cvt_f32 (s : option sx) (v : value) : option f32 :=
+  match v with
+  | ConstInt32 c =>
+    match s with
+    | Some sx_U => Some (Wasm_float.float_convert_ui32 f32m c)
+    | Some sx_S => Some (Wasm_float.float_convert_si32 f32m c)
+    | None => None
+    end
+  | ConstInt64 c =>
+    match s with
+    | Some sx_U => Some (Wasm_float.float_convert_ui64 f32m c)
+    | Some sx_S => Some (Wasm_float.float_convert_si64 f32m c)
+    | None => None
+    end
+  | ConstFloat32 c => None
+  | ConstFloat64 c => Some (wasm_demote c)
+  end.
+
+Definition cvt_f64 (s : option sx) (v : value) : option f64 :=
+  match v with
+  | ConstInt32 c =>
+    match s with
+    | Some sx_U => Some (Wasm_float.float_convert_ui32 f64m c)
+    | Some sx_S => Some (Wasm_float.float_convert_si32 f64m c)
+    | None => None
+    end
+  | ConstInt64 c =>
+    match s with
+    | Some sx_U => Some (Wasm_float.float_convert_ui64 f64m c)
+    | Some sx_S => Some (Wasm_float.float_convert_si64 f64m c)
+    | None => None
+    end
+  | ConstFloat32 c => Some (wasm_promote c)
+  | ConstFloat64 c => None
+  end.
+
+
+Definition cvt (t : value_type) (s : option sx) (v : value) : option value :=
+  match t with
+  | T_i32 => option_map ConstInt32 (cvt_i32 s v)
+  | T_i64 => option_map ConstInt64 (cvt_i64 s v)
+  | T_f32 => option_map ConstFloat32 (cvt_f32 s v)
+  | T_f64 => option_map ConstFloat64 (cvt_f64 s v)
+  end.
+
+Definition bits (v : value) : bytes :=
+  match v with
+  | ConstInt32 c => serialise_i32 c
+  | ConstInt64 c => serialise_i64 c
+  | ConstFloat32 c => serialise_f32 c
+  | ConstFloat64 c => serialise_f64 c
+  end.
+
+Definition bitzero (t : value_type) : value :=
+  match t with
+  | T_i32 => ConstInt32 (Wasm_int.int_zero i32m)
+  | T_i64 => ConstInt64 (Wasm_int.int_zero i64m)
+  | T_f32 => ConstFloat32 (Wasm_float.float_zero f32m)
+  | T_f64 => ConstFloat64 (Wasm_float.float_zero f64m)
+  end.
+
+Definition n_zeros (ts : list value_type) : list value :=
+  map bitzero ts.
+
+(* TODO: lots of lemmas *)
+
